{-# OPTIONS --without-K --exact-split --safe #-}

open import Prelude
open import UF-FunExt
open import ESIntervalObject
open import NaturalsAddition renaming (_+_ to _+ℕ_)
open import UF-Base

module IntervalObjectApproximation (fe : FunExt)
 (io : Interval-object fe 𝓤') (hd : has-double fe 𝓤' io) where

open basic-interval-object-development fe io hd hiding (−1 ; O ; +1)

data Vec (A : 𝓥 ̇) : ℕ → 𝓥 ̇ where
  [] : Vec A 0
  _∷_ : ∀ {n} → A → Vec A n → Vec A (succ n)

first-_ : {A : 𝓥 ̇ } (n : ℕ) → (ℕ → A) → Vec A n
(first- 0) a = []
(first- succ n) a = head a ∷ (first- n) (tail a)

append-one : {X : 𝓥 ̇ } {n : ℕ} → X → Vec X n → Vec X (succ n)
append-one {𝓥} {X} {0} y [] = y ∷ []
append-one {𝓥} {X} {succ n} y (x ∷ xs) = x ∷ append-one y xs

m : {n : ℕ} → Vec 𝕀 (succ n) → 𝕀
m {0} (x ∷ []) = x
m {succ n} (x ∷ xs) = x ⊕ m xs

n-approx : (x y : ℕ → 𝕀) (n : ℕ) → 𝓤' ̇
n-approx x y n = Σ (z , w) ꞉ 𝕀 × 𝕀
               , m (append-one z ((first- n) x))
               ≡ m (append-one w ((first- n) y))

approximation : 𝓤' ̇
approximation = (x y : ℕ → 𝕀) → Π (n-approx x y) → M x ≡ M y

multi-canc : (w z : 𝕀) (y : ℕ → 𝕀) (n : ℕ)
           → m (append-one w ((first- n) y))
           ≡ m (append-one z ((first- n) y))
           → w ≡ z
multi-canc w .w y zero refl = refl
multi-canc w z y (succ n) e
 = multi-canc w z (y ∘ succ) n (⊕-canc _ _ _ (⊕-comm ∙ e ∙ ⊕-comm))

one-sided-approx : (x : 𝕀) (y : ℕ → 𝕀)
                 → ((n : ℕ) → Σ w ꞉ 𝕀 , x ≡ m (append-one w ((first- n) y)))
                 → x ≡ M y
one-sided-approx x y f = M-prop₂ ws y γ where
  ws : ℕ → 𝕀
  ws 0 = x
  ws (succ i) = pr₁ (f (succ i))
  γ : (i : ℕ) → ws i ≡ (y i ⊕ ws (succ i))
  γ zero = pr₂ (f 1)
  γ (succ i) = multi-canc (ws (succ i)) (y (succ i) ⊕ ws (succ (succ i)))
               y (succ i) (pr₂ (f (succ i)) ⁻¹  ∙ (pr₂ (f (succ (succ i)))
             ∙ δ'' y (ws (succ (succ i))) i))
   where
    δ'' : (y : ℕ → 𝕀) (z : 𝕀) (i : ℕ)
        → m (append-one z ((first- (succ (succ i))) y))
        ≡ m (append-one (y (succ i) ⊕ z) ((first- (succ i)) y))
    δ'' y z zero = refl
    δ'' y z (succ i) = ap (y 0 ⊕_) (δ'' (y ∘ succ) z i)
    
_++_ : {n i : ℕ} {X : 𝓤 ̇ } → Vec X n → Vec X i → Vec X (n +ℕ i)
_++_ {_} {zero} {zero} {X} [] v₂ = v₂
_++_ {_} {zero} {succ i} {X} [] v₂
 = transport (Vec X) (ap succ (zero-left-neutral i ⁻¹)) v₂
_++_ {_} {succ n} {zero} {X} v₁ [] = v₁
_++_ {_} {succ n} {succ i} {X} (v ∷ v₁) v₂
 = transport (Vec X) (ap succ (δ n i)) (v ∷ (v₁ ++ v₂))
 where
  δ : ∀ n i → succ (n +ℕ i) ≡ succ n +ℕ i
  δ n zero = refl
  δ n (succ i) = ap succ (δ n i)

_++'_ : {n : ℕ} {X : 𝓤 ̇ } → Vec X n → (ℕ → X) → (ℕ → X)
[] ++' y = y
((x ∷ _) ++' _) zero = x
((_ ∷ v₁) ++' y) (succ n) = (v₁ ++' y) n

five : (n : ℕ) (a b c : ℕ → 𝕀) (e : 𝕀)
     → m (append-one e ((first- succ n) a))
       ⊕ M ((first- n) b ++' λ i → (c (succ (i +ℕ n))))
     ≡ M ((append-one (a n ⊕ e) ((first- n) λ i → a i ⊕ b i))
         ++' (λ i → c (succ (i +ℕ n))))
five zero a b c e = M-prop₁ _ ⁻¹
five (succ n) a b c e
 = ap ((a 0 ⊕ (a 1 ⊕ m (append-one e ((first- n) (a ∘ succ ∘ succ))))) ⊕_)
     (M-prop₁ ((first- succ n) b ++' (λ i → c (succ (i +ℕ succ n)))))
     ∙ ⊕-tran ∙ ap ((a 0 ⊕ b 0) ⊕_) (five n (tail a) (tail b) (tail c) e)
     ∙ M-prop₁ (append-one (a (succ n) ⊕ e)
         ((first- succ n) (λ i → a i ⊕ b i))
         ++' (λ i → c (succ (i +ℕ succ n)))) ⁻¹

equals : (x : ℕ → 𝕀) (n : ℕ)
       → M x
       ≡ M (append-one (x n) ((first- n) x) ++' (λ i → x (succ (i +ℕ n))))
equals x zero = M-prop₁ x
              ∙ M-prop₁ (append-one (x zero) ((first- zero) x) ++'
                          (λ i → x (succ (i +ℕ zero)))) ⁻¹
equals x (succ n) = M-prop₁ x
                  ∙ ap (x 0 ⊕_) (equals (tail x) n)
                  ∙ M-prop₁ (append-one (x (succ n)) ((first- succ n) x) ++'
                              (λ i → x (succ (i +ℕ succ n)))) ⁻¹

next : (x y : ℕ → 𝕀) (n : ℕ)
     → M (λ i → x i ⊕ y i)
     ≡ m (append-one (y n) ((first- succ n) x))
         ⊕ M (((first- n) y) ++' (λ i → (x (succ (i +ℕ n)))
                                      ⊕ (y (succ (i +ℕ n)))))
next x y n = equals (λ i → x i ⊕ y i) n
           ∙ five n x y (λ i → x i ⊕ y i) (y n) ⁻¹

equals2 : (x y : ℕ → 𝕀) (w : 𝕀) (n : ℕ)
        → (append-one w ((first- n) x)) ++' y
        ≡ ((first- n) x) ++' (w ∶∶ y)
equals2 x y w zero = dfunext (fe 𝓤₀ 𝓤') (induction refl λ _ _ → refl)
equals2 x y w (succ n) = dfunext (fe 𝓤₀ 𝓤') (induction refl
                           (λ k _ → happly (equals2 (tail x) y w n) k))

tail-_ : {X : 𝓤 ̇ } → ℕ → (ℕ → X) → (ℕ → X)
(tail- 0) α = α
(tail- succ n) α = tail ((tail- n) α)

M→m : (α : ℕ → 𝕀) (n : ℕ)
    → M α ≡ m (append-one (M ((tail- n) α)) ((first- n) α))
M→m α zero = refl
M→m α (succ n) = M-prop₁ α
               ∙ ap (α 0 ⊕_)
               (transport
                    (λ - → M (tail α)
                         ≡ m (append-one (M -) ((first- n) (tail α))))
                    (γ α n) (M→m (tail α) n))
  where
    γ : (α : ℕ → 𝕀) (n : ℕ) → ((tail- n) (tail α)) ≡ ((tail- succ n) α)
    γ α 0 = refl
    γ α (succ n) = ap tail (γ α n)

tl : {X : 𝓤 ̇} {m : ℕ} → Vec X (succ m) → Vec X m
tl (_ ∷ xs) = xs

tail-first' : {X : 𝓤 ̇ } {m : ℕ}
            → (a : Vec X (succ m)) (β : ℕ → X) (n : ℕ)
            → (tail- succ n) (a ++' β) ≡ (tail- n) (tl a ++' β)
tail-first' {X} {m} (_ ∷ xs) β 0 = refl
tail-first' {X} {m} (_ ∷ xs) β (succ n)
 = ap tail (tail-first' {X} {m} (_ ∷ xs) β n)

tail-first : {X : 𝓤 ̇ }
           → (α β : ℕ → X) (n : ℕ)
           → (tail- n) (((first- n) α) ++' β) ≡ β
tail-first α β zero = refl
tail-first α β (succ n)
 = tail-first' ((first- (succ n)) α) β n ∙ tail-first (tail α) β n

first-first : {X : 𝓤 ̇ }
            → (α β : ℕ → X) (n : ℕ)
            → ((first- n) ((first- n) α ++' β)) ≡ (first- n) α
first-first α β 0 = refl
first-first α β (succ n) = ap (α 0 ∷_) (first-first (tail α) β n)

approx-holds : approximation
approx-holds x y f = ⊕-canc (M x) (M y) (M (tail z)) seven
 where
  z w : ℕ → 𝕀
  z n = pr₁ (pr₁ (f n))
  w n = pr₂ (pr₁ (f n))
  w'' : (n : ℕ) → (ℕ → 𝕀)
  w'' n = (y n ⊕ pr₂ (pr₁ (f (succ n))))
       ∶∶ (λ i → x (succ (i +ℕ n)) ⊕ pr₁ (pr₁ (f (succ (succ (i +ℕ n))))))
  six : (n : ℕ) → m (append-one (z n) ((first- n) x))
                ≡ m (append-one (w n) ((first- n) y))
  six n = pr₂ (f n)
  γ' : (n : ℕ) → Σ w* ꞉ 𝕀 , M (λ i → x i ⊕ (tail z) i)
     ≡ m (append-one w* ((first- n) (λ i → y i ⊕ (tail z) i)))
  γ' n = M (w'' n)
       , (next x (tail z) n
       ∙ ap (_⊕ M ((first- n) (tail z) ++' (λ i → x (succ (i +ℕ n))
                                                ⊕ tail z (succ (i +ℕ n)))))
            (six (succ n))
       ∙ five n y (tail z) (λ i → x i ⊕ (tail z) i) (w (succ n))
       ∙ ap M (equals2 (λ i → y i ⊕ (tail z) i) ((λ i → x (succ (i +ℕ n))
                                                ⊕ (tail z) (succ (i +ℕ n))))
            (w'' n 0) n)
       ∙ M→m (((first- n) (λ i → y i ⊕ (tail z) i) ++' (w'' n))) n
       ∙ (ap (λ - → m (append-one (M -)
           ((first- n) ((first- n) (λ i → y i ⊕ (tail z) i) ++' (w'' n)))))
             (tail-first (λ i → y i ⊕ (tail z) i) (w'' n) n)
        ∙ ap (λ - → m (append-one (M (w'' n)) -))
           (first-first (λ i → y i ⊕ (tail z) i) (w'' n) n)))
  seven : M x ⊕ M (z ∘ succ) ≡ M y ⊕ M (z ∘ succ)
  seven = M-hom x (z ∘ succ)
        ∙ one-sided-approx
            (M (λ i → x i ⊕ pr₁ (pr₁ (f (succ i)))))
            (λ i → y i ⊕ z (succ i))
            γ'
        ∙ M-hom y (z ∘ succ) ⁻¹

n-approx' : (ℕ → 𝕀) → (ℕ → 𝕀) → ℕ → 𝓤' ̇
n-approx' x y n = Σ (z , w) ꞉ 𝕀 × 𝕀
                , m (append-one z ((first- (succ n)) x))
                ≡ m (append-one w ((first- (succ n)) y))

n-approx'→n-approx : (x y : ℕ → 𝕀) → Π (n-approx' x y) → Π (n-approx x y)
n-approx'→n-approx x y f zero = (u , u) , refl
n-approx'→n-approx x y f (succ n) = f n

fg-n-approx' : {X : 𝓥 ̇ } → (f g : X → ℕ → 𝕀) → ℕ → 𝓤' ⊔ 𝓥 ̇
fg-n-approx' f g n
 = (∀ x → n-approx' (f x) (g x) n) 
 → (∀ x → n-approx' (f x) (g x) (succ n)) 

fg-approx-holds : {X : 𝓥 ̇ } (f g : X → ℕ → 𝕀)
                → Π (fg-n-approx' f g)
                → ∀ x → M (f x) ≡ M (g x)
fg-approx-holds {_} {X} f g h x
 = approx-holds (f x) (g x) (n-approx'→n-approx (f x) (g x) (γ x))
 where
  γ : (x : X) → Π (n-approx' (f x) (g x))
  γ x 0 = (g x 0 , f x 0) , ⊕-comm
  γ x (succ n) = h n (λ y → γ y n) x
